wip

kosaraju-lean4/Tarjan/Env.lean
@@ -20,28 +20,48 @@ where
   num:  V -> Int
 
 def subenv [DirectedGraph V Graph] [BEq V] [LawfulBEq V] [DecidableEq V] (e e': Env V Graph graph) : Prop :=
-e.gray == e'.gray /\
+e.gray = e'.gray /\
 e.black ⊆ e'.black /\
 e.sccs ⊆ e'.sccs /\
 (∀ x, x ∈ e.stack -> e.num x = e'.num x) /\
 (∃ s, e'.stack = s ++ e.stack /\ ∀ x, x ∈ s → x ∈ e'.black)
 
+theorem subenv_trans [DirectedGraph V Graph] [BEq V] [LawfulBEq V] [DecidableEq V]
+                    {e1 e2 e3: Env V Graph graph}
+                    (h12 : subenv e1 e2)
+                    (h23 : subenv e2 e3)
+                    : subenv e1 e3 := by
+obtain ⟨ _,  _,  _, h₄, h₅, h₆, h₇⟩ := h12
+obtain ⟨k₁, k₂, k₃, k₄, k₅, k₆, k₇⟩ := h23
+repeat any_goals apply And.intro
+any_goals tauto
+any_goals simp_all
+use (k₅ ++ h₅)
+simp_all
+intros _ h
+cases h
+. apply k₇; assumption
+. apply k₂
+  apply h₇
+  assumption
+
+
 def wf_env [DirectedGraph V Graph] [BEq V] [LawfulBEq V] [DecidableEq V] (e : Env V Graph graph) : Prop :=
 let infty : Int := (DirectedGraph.vertices graph: List V).length
 let sccs_union : Finset V := List.foldl (· ∪ ·) ∅ e.sccs
-(∀ x, (-1 ≤ e.num x && e.num x < (e.sn: Int)) || e.num x == infty) /\
 e.sn = Finset.card (e.gray ∪ e.black) /\
+(∀ x, (-1 ≤ e.num x /\ e.num x < (e.sn: Int)) \/ e.num x == infty) /\
 (∀ x, e.num x = infty <-> x ∈ sccs_union) /\
 (∀ x, e.num x = (-1)  <-> ¬ x ∈ (e.gray ∪ e.black)) /\
-(∀ x y, x ∈ e.stack → y ∈ e.stack → e.num x <= e.num y ↔ precedes y x e.stack) /\
 (∀ x, x ∈ e.gray  -> x ∈ DirectedGraph.vertices graph) /\
 (∀ x, x ∈ e.black -> x ∈ DirectedGraph.vertices graph) /\
-e.black ∩ e.gray == ∅ /\
+e.black ∩ e.gray = ∅ /\
 sccs_union ⊆ e.black /\
 toFinset e.stack = (e.gray ∪ (e.black \ sccs_union)) /\
 no_black_to_white graph e.black e.gray /\
 simplelist e.stack /\
-(∀ x y, x ∈ e.stack -> y ∈ e.stack -> e.num x <= e.num y -> reachable graph x y) /\
+(∀ x y, x ∈ e.stack → y ∈ e.stack → e.num x <= e.num y ↔ precedes y x e.stack) /\
+(∀ x y, x ∈ e.stack → y ∈ e.stack → e.num x <= e.num y → reachable graph x y) /\
 (∀ y, y ∈ e.stack -> ∃ x, x ∈ e.gray /\ e.num x <= e.num y /\ reachable graph y x) /\
 (∀ cc, cc ∈ e.sccs <-> cc ⊆ e.black /\ is_scc graph cc) /\
 (∀ cc₁ cc₂, cc₁ ∈ e.sccs -> cc₂ ∈ e.sccs -> cc₁ = cc₂ \/ cc₁ ∩ cc₂ = ∅)
@@ -70,3 +90,44 @@ def num_of_reachable [DirectedGraph V Graph]
                      [BEq V] [LawfulBEq V] [DecidableEq V]
                      (n: Int) (x: V) (e: Env V Graph graph) : Prop :=
 ∃ y, y ∈ e.stack /\ n = e.num y /\ reachable graph x y
+
+private theorem num_lmem_inner [DirectedGraph V Graph]
+                               [BEq V] [LawfulBEq V] [DecidableEq V]
+                               {e : Env V Graph graph}
+                               (h : wf_env e)
+                               (x : V) :
+let infty : Int := (DirectedGraph.vertices graph: List V).length
+(¬ e.num x = -1) /\ (¬ e.num x = infty) <-> x ∈ toFinset e.stack := by
+obtain ⟨h₆, h₅, h₃, h₄, h₇, h₈, h₉, h₂, h, _⟩ := h
+rw [h]
+simp
+have h₅ := not_congr (h₃ x)
+have h₆ := not_congr (h₄ x)
+rw [h₅, h₆]
+simp
+constructor
+. tauto
+. intros h
+  cases h with
+  | inl h =>
+    constructor
+    . tauto
+    . intros h₁
+      specialize h₂ h₁
+      simp_all
+      have h : x ∈ e.black ∩ e.gray := by simp [Inter.inter]; tauto
+      rw [h₉] at h
+      tauto
+  | inr _ => tauto
+
+theorem num_lmem [DirectedGraph V Graph]
+                 [BEq V] [LawfulBEq V] [DecidableEq V]
+                 {e : Env V Graph graph}
+                 (h : wf_env e)
+                 (x : V) :
+let infty : Int := (DirectedGraph.vertices graph: List V).length
+(¬ e.num x = -1) /\ (¬ e.num x = infty) <-> x ∈ e.stack := by
+intros
+have h := num_lmem_inner h x
+simp at h
+rw [h]
